src/Comparse.Tactic.fst
@@ -3,3 +3,4 @@ module Comparse.Tactic
 include Comparse.Tactic.Attributes
 include Comparse.Tactic.GenerateParser
 include Comparse.Tactic.GenerateIsValidLemma
+include Comparse.Tactic.GenerateLengthLemma
